theories/Logic/inverse_ug_l.v
@@ -1,0 +1,715 @@
+From Cyclic_PA.Maths Require Import naturals.
+From Cyclic_PA.Maths Require Import lists.
+From Cyclic_PA.Maths Require Import ordinals.
+
+From Cyclic_PA.Logic Require Import definitions.
+From Cyclic_PA.Logic Require Import fol.
+From Cyclic_PA.Logic Require Import proof_trees.
+From Cyclic_PA.Logic Require Import substitute.
+
+Require Import List.
+Import ListNotations.
+
+Definition ug_left_inv_formula (phi A : formula) (v : ivar) (b : bool) : formula := formula_sub phi (univ v A) A b.
+
+Definition ug_left_inv_batch (gamma : list formula) (A : formula) (v : ivar) (S : subst_ind) : list formula := batch_sub gamma (univ v A) A S.
+
+Fixpoint ptree_ug_l_inv_fit
+  (P : ptree) (A : formula) (i : ivar) (S : subst_ind) : ptree :=
+let REC := (fun PT SI => (ptree_ug_l_inv_fit PT A i SI)) in
+match P, S with
+| bot, _ => P
+
+| pred vec pn pure, _ => P
+
+| equal v1 v2, _ => P
+
+| loop_head OC1 OC2 gamma delta sig P_Target, _ => loop_head OC1 OC2 (ug_left_inv_batch gamma A i S) delta sig (ptree_ug_l_inv_fit P_Target A i (list_filter S (sublist_filter form_eq_dec (map (fun lambda => sig_subst lambda (sig_generalise sig)) (ptree_left P_Target)) gamma)))
+
+| @con_l OC gamma delta phi v1 v2 alpha P', s1 :: s2 :: S' => @con_l OC (ug_left_inv_batch gamma A i S') delta (ug_left_inv_formula phi A i s2) v1 v2 alpha (REC P' (s1 :: s2 :: s2 :: S'))
+
+| @con_r OC gamma delta phi alpha P', _ => @con_r OC (ptree_left (REC P' S)) delta phi alpha (REC P' S)
+
+| @refl OC gamma delta v alpha P', _ => @refl OC (ug_left_inv_batch gamma A i S) delta v alpha (ptree_ug_l_inv_fit P' A i (false :: S))
+
+
+| @ex_l OC gamma delta n alpha P', _ => @ex_l OC (ptree_left (REC P' (unbury S n))) delta n alpha (REC P' (unbury S n))
+
+| @ex_r OC gamma delta n alpha P', _ => @ex_r OC (ptree_left (REC P' S)) delta n alpha (REC P' S)
+
+
+| @wkn_l OC gamma delta phi alpha P', s :: S' => @wkn_l OC (ug_left_inv_batch gamma A i S') delta (ug_left_inv_formula phi A i s) alpha (REC P' S')
+
+| @wkn_r OC gamma delta phi alpha P', _ => @wkn_r OC (ptree_left (REC P' S)) delta phi alpha (REC P' S)
+
+| @rst OC gamma delta kappa alpha P', _ => @rst OC (ptree_left (REC P' S)) delta kappa alpha (REC P' S)
+
+| @ug_l OC gamma delta phi v alpha P', s :: S' => match nat_eqb v i && form_eqb phi A, s with
+    | true, true => REC P' (false :: S')
+    | _, _ => let SI := (false :: S') in @ug_l OC (ug_left_inv_batch gamma A i S') delta phi v alpha (REC P' SI)
+    end
+
+| @ug_r OC gamma delta phi v alpha P', _ => @ug_r OC (ptree_left (REC P' S)) delta phi v alpha (REC P' S)
+
+| @bnd_l OC gamma delta phi lambda kappa alpha P', s :: S' => @bnd_l OC (ug_left_inv_batch gamma A i S') delta phi lambda kappa alpha (REC P' (false :: S'))
+
+| @bnd_r OC gamma delta phi lambda kappa alpha P', _ => @bnd_r OC (ptree_left (REC P' S)) delta phi lambda kappa alpha (REC P' S)
+
+| @imp_l OC gamma delta phi psi alpha1 alpha2 P1 P2, s :: S' =>  @imp_l OC (ug_left_inv_batch gamma A i S') delta phi psi alpha1 alpha2 (REC P1 (false :: S')) (REC P2 S')
+
+| @imp_r OC gamma delta phi psi alpha P', _ => @imp_r OC (ug_left_inv_batch gamma A i S) delta phi psi alpha (REC P' (false :: S))
+
+| @cut OC gamma delta phi alpha1 alpha2 P1 P2, _ => @cut OC (ug_left_inv_batch gamma A i S) delta phi alpha1 alpha2 (REC P1 S) (REC P2 (false :: S))
+
+| _ , _ => P
+end.
+
+Definition ptree_ug_l_inv (P : ptree) (A : formula) (i : ivar) (S : subst_ind) : ptree :=
+match nat_eqb (length (ptree_left P)) (length S) with
+| true => ptree_ug_l_inv_fit P A i S
+| false => P
+end.
+
+Lemma ptree_ug_l_inv_fit_true :
+    forall {P : ptree} {A : formula} {v : ivar},
+        forall {S : subst_ind},
+            nat_eqb (length (ptree_left P)) (length S) = true ->
+                (ptree_ug_l_inv_fit P A v S) = (ptree_ug_l_inv P A v S).
+Proof. intros P A v S EQ. unfold ptree_ug_l_inv. rewrite EQ. reflexivity. Qed.
+
+Lemma ptree_ug_l_inv_left :
+    forall (P : ptree) (A : formula) (v : ivar),
+        struct_valid P ->
+            forall (S : subst_ind),
+                ptree_left (ptree_ug_l_inv P A v S) =
+                    (ug_left_inv_batch (ptree_left P) A v S).
+Proof.
+intros P A v.
+induction P;
+try intros PSV S;
+unfold ptree_ug_l_inv;
+unfold ug_left_inv_batch, batch_sub;
+case nat_eqb eqn:EQ;
+try reflexivity;
+unfold ptree_ug_l_inv_fit;
+fold ptree_ug_l_inv_fit;
+unfold ptree_left in EQ;
+fold ptree_left in EQ.
+
+1-3 : destruct PSV.
+4 : destruct PSV as [[[[PSV [PG_app PD_app]] PL_app] Psig] PLoop].
+5-11 : destruct PSV as [[[[[PSV [PG_app PD_app]] PG] PD] POC] PDeg].
+12 : destruct PSV as [[[[[[[PSV [PG_app PD_app]] PG] PD] KNING] KNIND] [KIN POC]] PDeg].
+13-14 : destruct PSV as [[[[[PSV [PG_app PD_app]] PG] PD] POC] PDeg].
+15 : destruct PSV as [[[[[[PSV [PG_app PD_app]] PG] PD] POC] POC_rel] PDeg].
+16 : destruct PSV as [[[[[[PSV [PG_app PD_app]] PG] PD] [NEW [KIN POC]]] [NING NIND]] PDeg].
+17 : destruct PSV as [[[[[[[[[[P1SV P2SV] [PG_app PD_app]] P1G] P1D] P1OC] P2G] P2D] P2OC] PDeg1] PDeg2].
+18 : destruct PSV as [[[[[PSV [PG_app PD_app]] PG] PD] POC] PDeg].
+19 : destruct PSV as [[[[[[[[[[P1SV P2SV] [PG_app PD_app]] P1G] P1D] P1OC] P2G] P2D] P2OC] PDeg1] PDeg2].
+
+all : subst;
+      unfold ptree_left at 2;
+      try unfold ptree_left at 2;
+      unfold batch_sub_fit;
+      fold @batch_sub_fit.
+
+6,9,11,12,14,16 : rewrite (batch_sub_fit_true EQ);
+                  rewrite (ptree_ug_l_inv_fit_true EQ);
+                  apply (IHP PSV).
+
+1-3 : destruct S;
+      reflexivity.
+
+- rewrite (batch_sub_fit_true EQ).
+  reflexivity.
+
+- destruct S as [ | b1 [ | b2 S]].
+  inversion EQ.
+  inversion EQ.
+  rewrite batch_sub_fit_true, ptree_ug_l_inv_fit_true.
+  reflexivity.
+  rewrite PG.
+  apply EQ.
+  apply EQ.
+
+- rewrite (batch_sub_fit_true EQ).
+  reflexivity.
+
+- unfold ptree_left at 1.
+  fold (ptree_left (ptree_ug_l_inv_fit P A v (unbury S n))).
+  rewrite batch_sub_fit_true, ptree_ug_l_inv_fit_true, <- batch_bury_comm, (IHP PSV).
+  reflexivity.
+  rewrite bury_length, <- (@bury_unbury _ S n), bury_length in EQ.
+  apply EQ.
+  apply EQ.
+
+- destruct S as [ | b S].
+  inversion EQ.
+  unfold ptree_left at 1 2.
+  fold (ptree_left P).
+  unfold batch_sub_fit;
+  fold batch_sub_fit.  
+  rewrite batch_sub_fit_true.
+  reflexivity.
+  apply EQ.
+
+- destruct S as [ | b S].
+  inversion EQ.
+  unfold formula_sub, form_eqb;
+  fold form_eqb.
+  case (nat_eqb v0 v && form_eqb phi A) eqn:EQ'.
+  case b.
+  + apply and_bool_prop in EQ' as [EQ1 EQ2].
+    apply form_eqb_eq in EQ2.
+    subst.
+    rewrite ptree_ug_l_inv_fit_true, (IHP PSV), PG.
+    unfold ug_left_inv_batch, batch_sub, batch_sub_fit at 1;
+    fold batch_sub_fit.
+    unfold length in *;
+    fold (@length formula) (@length bool) in *.
+    rewrite EQ, formula_sub_false.
+    reflexivity.
+    rewrite PG.
+    apply EQ.
+  + unfold ptree_left.
+    rewrite batch_sub_fit_true.
+    reflexivity.
+    apply EQ.
+  + unfold ptree_left.
+    rewrite batch_sub_fit_true.
+    reflexivity.
+    apply EQ.
+
+- destruct S as [ | b S].
+  inversion EQ.
+  unfold ptree_left at 1, formula_sub, form_eqb.
+  rewrite batch_sub_fit_true.
+  reflexivity.
+  apply EQ.
+
+- destruct S as [ | b S].
+  inversion EQ.
+  unfold ptree_left at 1 2;
+  fold (ptree_left P2).
+  unfold batch_sub_fit;
+  fold batch_sub_fit.
+  rewrite batch_sub_fit_true.
+  reflexivity.
+  apply EQ.
+
+- rewrite (batch_sub_fit_true EQ).
+  reflexivity.
+
+- unfold ptree_left at 1.
+  fold (ptree_left P1).
+  rewrite batch_sub_fit_true.
+  reflexivity.
+  apply EQ.
+Qed.
+
+Lemma ptree_ug_l_inv_right :
+    forall (P : ptree) (A : formula) (v : ivar),
+        struct_valid P ->
+            forall (S : subst_ind),
+                ptree_right (ptree_ug_l_inv P A v S) =
+                   (ptree_right P).
+Proof.
+intros P A v.
+induction P;
+try intros PSV S;
+unfold ptree_ug_l_inv;
+unfold ug_left_inv_batch, batch_sub.
+
+1-3 : destruct PSV.
+4 : destruct PSV as [[[[PSV [PG_app PD_app]] PL_app] Psig] PLoop].
+5-11 : destruct PSV as [[[[[PSV [PG_app PD_app]] PG] PD] POC] PDeg].
+12 : destruct PSV as [[[[[[[PSV [PG_app PD_app]] PG] PD] KNING] KNIND] [KIN POC]] PDeg].
+13-14 : destruct PSV as [[[[[PSV [PG_app PD_app]] PG] PD] POC] PDeg].
+15 : destruct PSV as [[[[[[PSV [PG_app PD_app]] PG] PD] POC] POC_rel] PDeg].
+16 : destruct PSV as [[[[[[PSV [PG_app PD_app]] PG] PD] [NEW [KIN POC]]] [NING NIND]] PDeg].
+17 : destruct PSV as [[[[[[[[[[P1SV P2SV] [PG_app PD_app]] P1G] P1D] P1OC] P2G] P2D] P2OC] PDeg1] PDeg2].
+18 : destruct PSV as [[[[[PSV [PG_app PD_app]] PG] PD] POC] PDeg].
+19 : destruct PSV as [[[[[[[[[[P1SV P2SV] [PG_app PD_app]] P1G] P1D] P1OC] P2G] P2D] P2OC] PDeg1] PDeg2].
+
+all : subst; 
+      case nat_eqb eqn:EQ;
+      try reflexivity;
+      unfold ptree_ug_l_inv_fit;
+      fold ptree_ug_l_inv_fit;
+      unfold ptree_left in EQ;
+      fold ptree_left in EQ.
+
+2,4,5 : destruct S as [ | b S];
+        inversion EQ;
+        reflexivity.
+
+- destruct S as [ | b1 [ | b2 S]].
+  inversion EQ.
+  inversion EQ.
+  reflexivity.
+
+- destruct S as [ | b S].
+  inversion EQ.
+  case (nat_eqb v0 v && form_eqb phi A).
+  case b.
+  2,3 : reflexivity.
+  unfold ptree_right at 2.
+  rewrite ptree_ug_l_inv_fit_true.
+  apply (IHP PSV).
+  rewrite PG.
+  apply EQ.
+Qed.
+
+
+Lemma ptree_ug_l_inv_constraint :
+    forall (P : ptree) (A : formula) (v : ivar),
+        struct_valid P ->
+            forall (S : subst_ind),
+                ptree_constraint (ptree_ug_l_inv P A v S) =
+                   (ptree_constraint P).
+Proof.
+intros P A v.
+induction P;
+try intros PSV S;
+unfold ptree_ug_l_inv;
+unfold ug_left_inv_batch, batch_sub.
+
+1-3 : destruct PSV.
+4 : destruct PSV as [[[[PSV [PG_app PD_app]] PL_app] Psig] PLoop].
+5-11 : destruct PSV as [[[[[PSV [PG_app PD_app]] PG] PD] POC] PDeg].
+12 : destruct PSV as [[[[[[[PSV [PG_app PD_app]] PG] PD] KNING] KNIND] [KIN POC]] PDeg].
+13-14 : destruct PSV as [[[[[PSV [PG_app PD_app]] PG] PD] POC] PDeg].
+15 : destruct PSV as [[[[[[PSV [PG_app PD_app]] PG] PD] POC] POC_rel] PDeg].
+16 : destruct PSV as [[[[[[PSV [PG_app PD_app]] PG] PD] [NEW [KIN POC]]] [NING NIND]] PDeg].
+17 : destruct PSV as [[[[[[[[[[P1SV P2SV] [PG_app PD_app]] P1G] P1D] P1OC] P2G] P2D] P2OC] PDeg1] PDeg2].
+18 : destruct PSV as [[[[[PSV [PG_app PD_app]] PG] PD] POC] PDeg].
+19 : destruct PSV as [[[[[[[[[[P1SV P2SV] [PG_app PD_app]] P1G] P1D] P1OC] P2G] P2D] P2OC] PDeg1] PDeg2].
+
+all : subst; 
+      case nat_eqb eqn:EQ;
+      try reflexivity;
+      unfold ptree_ug_l_inv_fit;
+      fold ptree_ug_l_inv_fit;
+      unfold ptree_left in EQ;
+      fold ptree_left in EQ.
+
+2,4,5 : destruct S as [ | b S];
+        inversion EQ;
+        reflexivity.
+
+- destruct S as [ | b1 [ | b2 S]].
+  inversion EQ.
+  inversion EQ.
+  reflexivity.
+
+- destruct S as [ | b S].
+  inversion EQ.
+  case (nat_eqb v0 v && form_eqb phi A).
+  case b.
+  2,3 : reflexivity.
+  unfold ptree_constraint at 2.
+  rewrite ptree_ug_l_inv_fit_true.
+  apply (IHP PSV).
+  rewrite PG.
+  apply EQ.
+Qed.
+
+Lemma ptree_ug_l_inv_deg :
+    forall (P : ptree) (A : formula) (v : ivar),
+        struct_valid P ->
+            forall (S : subst_ind),
+                ptree_deg (ptree_ug_l_inv P A v S) =
+                   (ptree_deg P).
+Proof.
+intros P A v.
+induction P;
+try intros PSV S;
+unfold ptree_ug_l_inv;
+unfold ug_left_inv_batch, batch_sub.
+
+1-3 : destruct PSV.
+4 : destruct PSV as [[[[PSV [PG_app PD_app]] PL_app] Psig] PLoop].
+5-11 : destruct PSV as [[[[[PSV [PG_app PD_app]] PG] PD] POC] PDeg].
+12 : destruct PSV as [[[[[[[PSV [PG_app PD_app]] PG] PD] KNING] KNIND] [KIN POC]] PDeg].
+13-14 : destruct PSV as [[[[[PSV [PG_app PD_app]] PG] PD] POC] PDeg].
+15 : destruct PSV as [[[[[[PSV [PG_app PD_app]] PG] PD] POC] POC_rel] PDeg].
+16 : destruct PSV as [[[[[[PSV [PG_app PD_app]] PG] PD] [NEW [KIN POC]]] [NING NIND]] PDeg].
+17 : destruct PSV as [[[[[[[[[[P1SV P2SV] [PG_app PD_app]] P1G] P1D] P1OC] P2G] P2D] P2OC] PDeg1] PDeg2].
+18 : destruct PSV as [[[[[PSV [PG_app PD_app]] PG] PD] POC] PDeg].
+19 : destruct PSV as [[[[[[[[[[P1SV P2SV] [PG_app PD_app]] P1G] P1D] P1OC] P2G] P2D] P2OC] PDeg1] PDeg2].
+
+all : subst; 
+      case nat_eqb eqn:EQ;
+      try reflexivity;
+      unfold ptree_ug_l_inv_fit;
+      fold ptree_ug_l_inv_fit;
+      unfold ptree_left in EQ;
+      fold ptree_left in EQ.
+
+2,4,5 : destruct S as [ | b S];
+        inversion EQ;
+        reflexivity.
+
+- destruct S as [ | b1 [ | b2 S]].
+  inversion EQ.
+  inversion EQ.
+  reflexivity.
+
+- destruct S as [ | b S].
+  inversion EQ.
+  case (nat_eqb v0 v && form_eqb phi A).
+  case b.
+  2,3 : reflexivity.
+  unfold ptree_deg at 2.
+  rewrite ptree_ug_l_inv_fit_true.
+  apply (IHP PSV).
+  rewrite PG.
+  apply EQ.
+Qed.
+
+Lemma ug_l_formula_inv_vars :
+    forall (phi : formula) (A : formula) (v : ivar),
+        forall (b : bool),
+            vars_in (ug_left_inv_formula phi A v b) =
+                vars_in phi.
+Proof.
+intros phi A v b.
+unfold ug_left_inv_formula, formula_sub.
+case form_eqb eqn:EQf.
+case b.
+apply form_eqb_eq in EQf.
+subst.
+all : reflexivity.
+Qed.
+
+Lemma ptree_ug_l_inv_vars :
+    forall (gamma : list formula) (A : formula) (v : ivar),
+        forall (S : subst_ind),
+            flat_map vars_in (ug_left_inv_batch gamma A v S) =
+                flat_map vars_in gamma.
+Proof.
+induction gamma;
+intros A v S;
+unfold ug_left_inv_batch, batch_sub, batch_sub_fit;
+fold batch_sub_fit;
+destruct S;
+unfold length, nat_eqb;
+fold (@length formula) (@length bool) nat_eqb.
+1-3 : reflexivity.
+case nat_eqb eqn:EQn.
+unfold flat_map;
+fold (flat_map vars_in).
+rewrite (batch_sub_fit_true EQn).
+fold (ug_left_inv_batch gamma A v S).
+rewrite IHgamma.
+unfold formula_sub.
+case form_eqb eqn:EQf.
+case b.
+apply form_eqb_eq in EQf.
+subst.
+all : reflexivity.
+Qed.
+
+Lemma ptree_ug_l_inv_bot :
+    forall (phi : formula) (v : ivar) (S : subst_ind),
+        ptree_ug_l_inv bot phi v S = bot.
+Proof.
+intros phi v S.
+unfold ptree_ug_l_inv, ptree_ug_l_inv_fit.
+case (nat_eqb);
+reflexivity.
+Qed.
+
+Lemma ptree_ug_l_inv_struct :
+    forall (P : ptree) (A : formula) (v : ivar),
+        struct_valid P ->
+            forall (S : subst_ind),
+                struct_valid (ptree_ug_l_inv P A v S).
+Proof.
+intros P.
+induction P;
+try intros AF vf PSV S;
+unfold ptree_ug_l_inv;
+unfold ug_left_inv_batch, batch_sub;
+case nat_eqb eqn:EQ;
+try apply PSV.
+
+all : unfold ptree_ug_l_inv_fit;
+      fold ptree_ug_l_inv_fit.
+
+14 :  destruct S as [ | b S];
+      try apply PSV.
+
+12 :  destruct S as [ | b S];
+      try apply PSV.
+
+10 :  destruct S as [ | b S];
+      try apply PSV.
+
+7 : destruct S as [ | b S];
+    try apply PSV.
+
+2 : destruct S as [ | b1 [ | b2 S]];
+    try apply PSV.
+
+1 : destruct PSV as [[[[[PSV [PG_app PD_app]] PL_app] PL_OC] Psig] PLoop].
+2-8 : destruct PSV as [[[[[PSV [PG_app PD_app]] PG] PD] POC] PDeg].
+9 : destruct PSV as [[[[[[[PSV [PG_app PD_app]] PG] PD] KNING] KNIND] [KIN POC]] PDeg].
+10-11 : destruct PSV as [[[[[PSV [PG_app PD_app]] PG] PD] POC] PDeg].
+12 : destruct PSV as [[[[[[PSV [PG_app PD_app]] PG] PD] POC] POC_rel] PDeg].
+13 : destruct PSV as [[[[[[PSV [PG_app PD_app]] PG] PD] FRESH] [NING NIND]] PDeg].
+14 : destruct PSV as [[[[[[[[[[P1SV P2SV] [PG_app PD_app]] P1G] P1D] P1OC] P2G] P2D] P2OC] PDeg1] PDeg2].
+15 : destruct PSV as [[[[[PSV [PG_app PD_app]] PG] PD] POC] PDeg].
+16 : destruct PSV as [[[[[[[[[[P1SV P2SV] [PG_app PD_app]] P1G] P1D] P1OC] P2G] P2D] P2OC] PDeg1] PDeg2].
+
+all : subst.
+
+10 :  case (nat_eqb v vf && form_eqb phi AF) eqn:EQfn;
+      case b.
+
+1 : { destruct Psig as [[OC_Sub [Order Coherent]] [SUBG SUBD]].
+      rewrite ptree_ug_l_inv_fit_true.
+      2 : { rewrite sublist_count_length, sublist_filter_true, map_length.
+            apply nat_eqb_refl.
+            apply SUBG.
+            rewrite sublist_filter_length.
+            apply (eq_sym (nat_eqb_eq _ _ EQ)).
+            apply SUBG. }
+      repeat split;
+      try rewrite P1G;
+      try rewrite P2G;
+      try apply EQ;
+      try unfold ptree_left at 1 in EQ;
+      try rewrite bury_length, <- (@bury_unbury _ S n), bury_length in EQ;
+      try apply EQ;
+      repeat split;
+      try rewrite ptree_ug_l_inv_constraint;
+      try apply ptree_ug_l_inv_deg;
+      try rewrite ptree_ug_l_inv_left;
+      try rewrite PG;
+      try rewrite P1G;
+      try rewrite P2G;
+      unfold flat_map;
+      fold (flat_map vars_in);
+      try rewrite ptree_ug_l_inv_vars;
+      try rewrite ug_l_formula_inv_vars;
+      unfold ug_left_inv_batch;
+      try rewrite batch_sub_false_head;
+      try rewrite ptree_ug_l_inv_right;
+      try apply Order;
+      try assumption;
+      try apply (IHP _ _ PSV);
+      try apply (IHP1 _ _ P1SV);
+      try apply (IHP2 _ _ P2SV);
+      try reflexivity.
+      - destruct PL_OC as [EQ' | PL_OC].
+        subst.
+        left.
+        apply ptree_ug_l_inv_bot.
+        right.
+        apply PL_OC.
+      - pose proof (batch_sub_sublist _ _ (univ vf AF) AF S SUBG (nat_eqb_eq _ _ EQ)).
+        rewrite map_batch_sub.
+        + admit.
+        + intros phi1 phi2.
+          split;
+          intros EQ'.
+          subst.
+          reflexivity.
+          
+
+        apply coherent_is_injective.
+        apply batch_sub_sublist. _ _ _ _ _ SUBG (nat_eqb_eq _ _ EQ)). *)
+        admit.
+      - admit.
+}
+
+all : repeat rewrite ptree_ug_l_inv_fit_true;
+      try rewrite PG;
+      try rewrite P1G;
+      try rewrite P2G;
+      try apply EQ;
+      unfold ptree_left at 1 in EQ;
+      try rewrite bury_length, <- (@bury_unbury _ S n), bury_length in EQ;
+      try apply EQ;
+      repeat split;
+      try rewrite ptree_ug_l_inv_constraint;
+      try apply ptree_ug_l_inv_deg;
+      try rewrite ptree_ug_l_inv_left;
+      try rewrite PG;
+      try rewrite P1G;
+      try rewrite P2G;
+      unfold flat_map;
+      fold (flat_map vars_in);
+      try rewrite ptree_ug_l_inv_vars;
+      try rewrite ug_l_formula_inv_vars;
+      unfold ug_left_inv_batch;
+      try rewrite batch_sub_false_head;
+      try rewrite ptree_ug_l_inv_right;
+      try assumption;
+      try apply (IHP _ _ PSV);
+      try apply (IHP1 _ _ P1SV);
+      try apply (IHP2 _ _ P2SV);
+      try reflexivity.
+
+1 : unfold batch_sub, batch_sub_fit;
+    fold batch_sub_fit.
+    unfold length in *;
+    fold (@length formula) (@length bool) in *;
+    unfold nat_eqb in *;
+    fold nat_eqb in *.
+    rewrite EQ.
+    unfold formula_sub at 1, form_eqb, ug_left_inv_formula.
+    admit.
+Qed.
+
+Lemma demorgan1_valid :
+    forall (P : ptree) (E F : formula),
+        valid P ->
+            forall (S : subst_ind),
+                subst_ind_fit (ptree_formula P) S = true ->
+                    valid (demorgan1_sub_ptree P E F S).
+Proof.
+intros P E F [PSV PAX].
+induction P; try intros S FS;
+unfold demorgan1_sub_ptree;
+rewrite FS;
+unfold ptree_formula in *; fold ptree_formula in *;
+unfold demorgan1_sub_ptree_fit; fold demorgan1_sub_ptree_fit.
+
+all : try apply (PSV,PAX).
+
+1 : { repeat split.
+      rewrite dem1_axiom_id;
+      apply PAX.
+      apply or_introl, eq_refl. }
+
+  1 : destruct PSV as [PSV DU].
+  2 : destruct PSV as [[PSV OU] NO].
+  3-10 : destruct PSV as [[[PF PSV] PD] PO].
+  11 : destruct PSV as [[[[PF PSV] PD] PO] FC].
+  12-16: destruct PSV as [[[[[[[P1F P1SV] P1D] P1O] P2F] P2SV] P2D] P2O].
+  17: destruct PSV as [[[[[[[[P1F P1SV] P1D] P1O] P2F] P2SV] P2D] P2O] INA].
+
+  3-6,8-13,16,17 : 
+      destruct S; inversion FS as [FS'];
+      try destruct (and_bool_prop _ _ FS') as [FS1 FS2].
+
+  4-6,13 :  destruct S1; inversion FS' as [FS''];
+            try destruct (and_bool_prop _ _ FS1) as [FS1_1 FS1_2].
+
+  6 : destruct S1_1; inversion FS'' as [FS'''];
+      destruct (and_bool_prop _ _ FS1_1) as [FS1_1_1 FS1_1_2].
+
+  7,8,13,14 :
+      case (form_eqb a E) eqn:EQ1;
+      case (form_eqb b F) eqn:EQ2;
+      unfold ptree_deg; fold ptree_deg;
+      try apply (PSV,PAX).
+
+11,19 : case (nat_eqb d1 (Nat.max d1 d2)) eqn:EQ.
+
+
+all : unfold node_extract in *;
+      fold node_extract in *;
+      try apply form_eqb_eq in EQ1;
+      try destruct EQ1;
+      try apply form_eqb_eq in EQ2;
+      try destruct EQ2;
+      repeat rewrite demorgan1_ptree_formula_true;
+      repeat split;
+      try apply IHP;
+      try apply (IHP1 P1SV);
+      try apply (IHP2 P2SV);
+      unfold ptree_deg; fold ptree_deg;
+      try rewrite demorgan1_ptree_deg;
+      try rewrite demorgan1_ptree_ord;
+      try apply ptree_ord_nf_struct;
+      unfold ptree_ord; fold ptree_ord;
+      try rewrite demorgan1_ptree_formula;
+      try rewrite PF;
+      try rewrite P1F;
+      try rewrite P2F;
+      repeat split;
+      unfold demorgan1_sub_formula;
+      repeat rewrite formula_sub_ind_lor;
+      try rewrite formula_sub_ind_0;
+      try rewrite non_target_sub;
+      try rewrite non_target_sub_term;
+      try apply PSV;
+      try apply PAX;
+      try apply PD;
+      try rewrite PO;
+      try apply P1SV;
+      try rewrite P1D in *;
+      try rewrite P1O;
+      try apply P2SV;
+      try rewrite P2D in *;
+      try rewrite P2O;
+      try apply FS;
+      try apply DU;
+      try apply OU;
+      try apply NO;
+      try apply INA;
+      try rewrite PF;
+      try rewrite P1F;
+      try rewrite P2F;
+      unfold subst_ind_fit, non_target;
+      fold subst_ind_fit non_target;
+      try rewrite non_target_fit;
+      try rewrite non_target_sub_fit;
+      try rewrite FS;
+      try rewrite FS';
+      try rewrite FS'';
+      try rewrite FS1;
+      try rewrite FS1_1;
+      try rewrite FS1_2;
+      try rewrite FS1_1_1;
+      try rewrite FS1_1_2;
+      try rewrite FS2;
+      unfold "&&";
+      try reflexivity;
+      try apply (fun B INB => PAX B (in_or_app _ _ _ (or_introl INB)));
+      try apply (fun B INB => PAX B (in_or_app _ _ _ (or_intror INB)));
+      try apply max_lem1;
+      try apply EQ;
+      try apply ord_lt_max_succ_l;
+      try reflexivity.
+
+  8 : { intros B INB.
+        rewrite closed_free_list in INB.
+        inversion INB.
+        apply formula_sub_ind_closed.
+        apply (valid_closed_formula PAX FC).
+        intros CEF.
+        apply and_bool_prop in CEF as [CE CF].
+        apply CE. }
+
+  all : unfold node_extract in *;
+        fold node_extract in *;
+        intros A IN;
+        try apply in_app_or in IN as [IN1 | IN2];
+        try apply (fun FSUB => dem1_all_ax_trans _ _ _ _ P1SV FSUB (fun B INB1 => PAX B (in_or_app _ _ _ (or_introl INB1))) _ IN1);
+        try apply (fun FSUB => dem1_all_ax_trans _ _ _ _ P2SV FSUB (fun B INB2 => PAX B (in_or_app _ _ _ (or_intror INB2))) _ IN2);
+        try apply (PAX _ (in_or_app _ _ _ (or_introl IN1)));
+        try apply (PAX _ (in_or_app _ _ _ (or_intror IN2)));
+        try rewrite P1F;
+        try rewrite P2F;
+        unfold subst_ind_fit;
+        fold subst_ind_fit;
+        try rewrite FS;
+        try rewrite FS1;
+        try rewrite FS2;
+        try rewrite non_target_fit;
+        try reflexivity.
+
+  all : try apply (PAX _ (in_or_app _ _ _ (or_intror IN)));
+        try apply in_app_or in IN as [IN1 | IN2];
+        try apply (PAX _ (in_or_app _ _ _ (or_introl IN1)));
+        try apply (fun FSUB => dem1_all_ax_trans _ _ _ _ P1SV FSUB (fun B INB => PAX B (in_or_app _ _ _ (or_intror INB))) _ IN2);
+        try rewrite P1F;
+        unfold subst_ind_fit;
+        fold subst_ind_fit;
+        try rewrite FS1, non_target_sub_fit;
+        try reflexivity.
+Qed.
